Migrate Imp.v to version 6.7.1 (2025-01-13)

lf/Imp.v
@@ -22,14 +22,15 @@
     reasoning about imperative programs. *)
 
 Set Warnings "-notation-overridden,-parsing,-deprecated-hint-without-locality".
-From Coq Require Import Bool.Bool.
+From Coq Require Import Bool.
 From Coq Require Import Init.Nat.
-From Coq Require Import Arith.Arith.
-From Coq Require Import Arith.EqNat. Import Nat.
+From Coq Require Import Arith.
+From Coq Require Import EqNat. Import Nat.
 From Coq Require Import Lia.
-From Coq Require Import Lists.List. Import ListNotations.
+From Coq Require Import List. Import ListNotations.
 From Coq Require Import Strings.String.
 From LF Require Import Maps.
+Set Default Goal Selector "!".
 
 (* ################################################################# *)
 (** * Arithmetic and Boolean Expressions *)
@@ -242,17 +243,16 @@ Proof.
 (** If [T] is a tactic, then [try T] is a tactic that is just like [T]
     except that, if [T] fails, [try T] _successfully_ does nothing at
     all (rather than failing). *)
-
-Theorem silly1 : forall ae, aeval ae = aeval ae.
-Proof.
-    try reflexivity. (* This just does [reflexivity]. *)
-Qed.
-
-Theorem silly2 : forall (P : Prop), P -> P.
+Theorem silly1 : forall (P : Prop), P -> P.
 Proof.
   intros P HP.
   try reflexivity. (* Plain [reflexivity] would have failed. *)
   apply HP. (* We can still finish the proof in some other way. *)
+Qed.
+
+Theorem silly2 : forall ae, aeval ae = aeval ae.
+Proof.
+    try reflexivity. (* This just does [reflexivity]. *)
 Qed.
 
 (** There is not much reason to use [try] in completely manual
@@ -472,15 +472,28 @@ Fixpoint optimize_0plus_b (b : bexp) : bexp
   | BNeq a1 a2  => BNeq (optimize_0plus a1) (optimize_0plus a2)
   | BLe a1 a2   => BLe (optimize_0plus a1) (optimize_0plus a2)
   | BGt a1 a2   => BGt (optimize_0plus a1) (optimize_0plus a2)
-  | other       => other
+  | BNot b      => BNot (optimize_0plus_b b)
+  | BAnd b1 b2  => BAnd (optimize_0plus_b b1) (optimize_0plus_b b2)
   end.
+
+Example optimize_0plus_b_test1:
+  optimize_0plus_b (BNot (BGt (APlus (ANum 0) (ANum 4)) (ANum 8))) =
+                   (BNot (BGt (ANum 4) (ANum 8))).
+Proof. reflexivity. Qed.
+
+Example optimize_0plus_b_test2:
+  optimize_0plus_b (BAnd (BLe (APlus (ANum 0) (ANum 4)) (ANum 5)) BTrue) =
+                   (BAnd (BLe (ANum 4) (ANum 5)) BTrue).
+Proof. reflexivity. Qed.
 
 Theorem optimize_0plus_b_sound : forall b,
   beval (optimize_0plus_b b) = beval b.
 Proof.
   intros b.
-  destruct b;
+  induction b;
   try (simpl; repeat (rewrite optimize_0plus_sound); reflexivity).
+  - simpl. f_equal. apply IHb.
+  - simpl. rewrite IHb1. rewrite IHb2. reflexivity.
 Qed.
 (** [] *)
 
@@ -539,7 +552,9 @@ Proof.
     + destruct n.
       * reflexivity.
       * destruct (optimize a2).
-        ** destruct n0. rewrite add_0_r. reflexivity. reflexivity.
+        ** destruct n0.
+           *** rewrite add_0_r. reflexivity.
+           *** reflexivity.
         ** reflexivity.
         ** reflexivity.
         ** reflexivity.
@@ -548,7 +563,9 @@ Proof.
     + destruct n.
       * reflexivity.
       * destruct (optimize a2).
-        ** destruct n0. reflexivity. reflexivity.
+        ** destruct n0.
+           *** reflexivity.
+           *** reflexivity.
         ** reflexivity.
         ** reflexivity.
         ** reflexivity.
@@ -559,7 +576,11 @@ Proof.
       * destruct n.
         ** simpl. rewrite add_0_r. reflexivity.
         ** destruct (optimize a2).
-          *** destruct n0. rewrite mul_0_r. reflexivity. destruct n0. rewrite mul_1_r. reflexivity. reflexivity.
+          *** destruct n0.
+              **** rewrite mul_0_r. reflexivity.
+              **** destruct n0.
+                   ***** rewrite mul_1_r. reflexivity.
+                   ***** reflexivity.
           *** reflexivity.
           *** reflexivity.
           *** reflexivity.
@@ -594,7 +615,8 @@ Qed.
 
     Here's an example [Ltac] script called [invert]. *)
 
-Ltac invert H := inversion H; subst; clear H.
+Ltac invert H :=
+  inversion H; subst; clear H.
 
 (** This defines a new tactic called [invert] that takes a hypothesis
     [H] as an argument and performs the sequence of commands
@@ -611,8 +633,8 @@ Qed.
 (* ================================================================= *)
 (** ** The [lia] Tactic *)
 
-(** The [lia] tactic implements a decision procedure for a subset of
-    first-order logic called _Presburger arithmetic_.
+(** The [lia] tactic implements a decision procedure for integer linear
+    arithmetic, a subset of propositional logic and arithmetic.
 
     If the goal is a universally quantified formula made out of
 
@@ -688,10 +710,10 @@ Qed.
 (** * Evaluation as a Relation *)
 
 (** We have presented [aeval] and [beval] as functions defined by
-    [Fixpoint]s.  Another way to think about evaluation -- one that we
-    will see is often more flexible -- is as a _relation_ between
-    expressions and their values.  This leads naturally to [Inductive]
-    definitions like the following... *)
+    [Fixpoint]s.  Another way to think about evaluation -- one that is
+    often more flexible -- is as a _relation_ between expressions and
+    their values.  This perspective leads to [Inductive] definitions
+    like the following... *)
 
 Module aevalR_first_try.
 
@@ -780,16 +802,16 @@ Inductive aevalR : aexp -> nat -> Prop :=
 (** In informal discussions, it is convenient to write the rules
     for [aevalR] and similar relations in the more readable graphical
     form of _inference rules_, where the premises above the line
-    justify the conclusion below the line. *)
+    justify the conclusion below the line.
 
-(** For example, the constructor [E_APlus]...
+    For example, the constructor [E_APlus]...
 
       | E_APlus : forall (e1 e2 : aexp) (n1 n2 : nat),
           aevalR e1 n1 ->
           aevalR e2 n2 ->
           aevalR (APlus e1 e2) (n1 + n2)
 
-    ...would be written like this as an inference rule:
+    ...can be written like this as an inference rule:
 
                                e1 ==> n1
                                e2 ==> n2
@@ -816,8 +838,8 @@ Inductive aevalR : aexp -> nat -> Prop :=
     indicated by saying something like "Let [aevalR] be the smallest
     relation closed under the following rules...". *)
 
-(** For example, [==>] is the smallest relation closed under these
-    rules:
+(** For example, we could define [==>] as the smallest relation
+    closed under these rules:
 
                              -----------                               (E_ANum)
                              ANum n ==> n
@@ -868,45 +890,45 @@ Definition manual_grade_for_beval_rules : option (nat*string) := None.
 (** It is straightforward to prove that the relational and functional
     definitions of evaluation agree: *)
 
-Theorem aeval_iff_aevalR : forall a n,
+Theorem aevalR_iff_aeval : forall a n,
   (a ==> n) <-> aeval a = n.
 Proof.
- split.
- - (* -> *)
-   intros H.
-   induction H; simpl.
-   + (* E_ANum *)
-     reflexivity.
-   + (* E_APlus *)
-     rewrite IHaevalR1.  rewrite IHaevalR2.  reflexivity.
-   + (* E_AMinus *)
-     rewrite IHaevalR1.  rewrite IHaevalR2.  reflexivity.
-   + (* E_AMult *)
-     rewrite IHaevalR1.  rewrite IHaevalR2.  reflexivity.
- - (* <- *)
-   generalize dependent n.
-   induction a;
-      simpl; intros; subst.
-   + (* ANum *)
-     apply E_ANum.
-   + (* APlus *)
-     apply E_APlus.
-      apply IHa1. reflexivity.
-      apply IHa2. reflexivity.
-   + (* AMinus *)
-     apply E_AMinus.
-      apply IHa1. reflexivity.
-      apply IHa2. reflexivity.
-   + (* AMult *)
-     apply E_AMult.
-      apply IHa1. reflexivity.
-      apply IHa2. reflexivity.
+  split.
+  - (* -> *)
+    intros H.
+    induction H; simpl.
+    + (* E_ANum *)
+      reflexivity.
+    + (* E_APlus *)
+      rewrite IHaevalR1.  rewrite IHaevalR2.  reflexivity.
+    + (* E_AMinus *)
+      rewrite IHaevalR1.  rewrite IHaevalR2.  reflexivity.
+    + (* E_AMult *)
+      rewrite IHaevalR1.  rewrite IHaevalR2.  reflexivity.
+  - (* <- *)
+    generalize dependent n.
+    induction a;
+       simpl; intros; subst.
+    + (* ANum *)
+      apply E_ANum.
+    + (* APlus *)
+      apply E_APlus.
+      * apply IHa1. reflexivity.
+      * apply IHa2. reflexivity.
+    + (* AMinus *)
+      apply E_AMinus.
+      * apply IHa1. reflexivity.
+      * apply IHa2. reflexivity.
+    + (* AMult *)
+      apply E_AMult.
+      * apply IHa1. reflexivity.
+      * apply IHa2. reflexivity.
 Qed.
 
 (** Again, we can make the proof quite a bit shorter using some
-    tactics. *)
+    tacticals. *)
 
-Theorem aeval_iff_aevalR' : forall a n,
+Theorem aevalR_iff_aeval' : forall a n,
   (a ==> n) <-> aeval a = n.
 Proof.
   (* WORKED IN CLASS *)
@@ -937,7 +959,7 @@ Inductive bevalR: bexp -> bool -> Prop :=
 where "e '==>b' b" := (bevalR e b) : type_scope
 .
 
-Lemma beval_iff_bevalR : forall b bv,
+Lemma bevalR_iff_beval : forall b bv,
   b ==>b bv <-> beval b = bv.
 Proof.
   intros.
@@ -945,17 +967,17 @@ Proof.
   - intros H.
     induction H;
       simpl;
-      try (apply aeval_iff_aevalR in H1; apply aeval_iff_aevalR in H2);
+      try (apply aevalR_iff_aeval in H1; apply aevalR_iff_aeval in H2);
       subst;
       reflexivity.
   - intros H.
     destruct b;
       subst; constructor;
-      try (apply aeval_iff_aevalR; reflexivity);
+      try (apply aevalR_iff_aeval; reflexivity);
       [ | rename b1 into b | rename b2 into b ];
       induction b;
       constructor;
-      try (apply aeval_iff_aevalR; reflexivity);
+      try (apply aevalR_iff_aeval; reflexivity);
       try (apply IHb);
       try (apply IHb1);
       try (apply IHb2).
@@ -1009,8 +1031,9 @@ Inductive aevalR : aexp -> nat -> Prop :=
 
 where "a '==>' n" := (aevalR a n) : type_scope.
 
-(** Notice that the evaluation relation has become _partial_: There
-    are some inputs for which it does not specify an output. *)
+(** Notice that this evaluation relation corresponds to a _partial_
+    function: There are some inputs for which it does not specify an
+    output. *)
 
 End aevalR_division.
 
@@ -1092,8 +1115,10 @@ End aevalR_extended.
 
 (** Let's return to defining Imp, where the next thing we need to do
     is to enrich our arithmetic and boolean expressions with
-    variables. To keep things simple, we'll assume that all variables
-    are global and that they only hold numbers. *)
+    variables.
+
+    To keep things simple, we'll assume that all variables are global
+    and that they only hold numbers. *)
 
 (* ================================================================= *)
 (** ** States *)
@@ -1156,19 +1181,22 @@ Inductive bexp : Type :=
 (** ** Notations *)
 
 (** To make Imp programs easier to read and write, we introduce some
-    notations and implicit coercions.  You do not need to understand
-    exactly what these declarations do.  Briefly, though:
+    notations and implicit coercions.  *)
+
+(** You do not need to understand exactly what these declarations do.
+
+    Briefly, though:
        - The [Coercion] declaration stipulates that a function (or
          constructor) can be implicitly used by the type system to
          coerce a value of the input type to a value of the output
          type.  For instance, the coercion declaration for [AId]
          allows us to use plain strings when an [aexp] is expected;
          the string will implicitly be wrapped with [AId].
-       - [Declare Custom Entry com] tells Coq to create a new
-         "custom grammar" for parsing Imp expressions and
-         programs. The first notation declaration after this tells Coq
-         that anything between [<{] and [}>] should be parsed using
-         the Imp grammar. Again, it is not necessary to understand the
+       - [Declare Custom Entry com] tells Coq to create a new "custom
+         grammar" for parsing Imp expressions and programs. The first
+         notation declaration after this tells Coq that anything
+         between [<{] and [}>] should be parsed using the Imp
+         grammar. Again, it is not necessary to understand the
          details, but it is important to recognize that we are
          defining _new_ interpretations for some familiar operators
          like [+], [-], [*], [=], [<=], etc., when they occur between
@@ -1179,8 +1207,11 @@ Coercion ANum : nat >-> aexp.
 
 Declare Custom Entry com.
 Declare Scope com_scope.
+Declare Custom Entry com_aux.
 
-Notation "<{ e }>" := e (at level 0, e custom com at level 99) : com_scope.
+Notation "<{ e }>" := e (e custom com_aux) : com_scope.
+Notation "e" := e (in custom com_aux at level 0, e custom com) : com_scope.
+
 Notation "( x )" := x (in custom com, x at level 99) : com_scope.
 Notation "x" := x (in custom com at level 0, x constr at level 0) : com_scope.
 Notation "f x .. y" := (.. (f x) .. y)
@@ -1216,7 +1247,8 @@ Definition example_bexp : bexp := <{ true && ~(X <= 4) }>.
     handle variables in the obvious way, taking a state [st] as an
     extra argument: *)
 
-Fixpoint aeval (st : state) (* <--- NEW *) (a : aexp) : nat :=
+Fixpoint aeval (st : state) (* <--- NEW *)
+               (a : aexp) : nat :=
   match a with
   | ANum n => n
   | AId x => st x                                (* <--- NEW *)
@@ -1225,7 +1257,8 @@ Fixpoint aeval (st : state) (* <--- NEW *) (a : aexp) : nat :=
   | <{a1 * a2}> => (aeval st a1) * (aeval st a2)
   end.
 
-Fixpoint beval (st : state) (* <--- NEW *) (b : bexp) : bool :=
+Fixpoint beval (st : state) (* <--- NEW *)
+               (b : bexp) : bool :=
   match b with
   | <{true}>      => true
   | <{false}>     => false
@@ -1264,7 +1297,7 @@ Proof. reflexivity. Qed.
 (* ################################################################# *)
 (** * Commands *)
 
-(** Now we are ready define the syntax and behavior of Imp
+(** Now we are ready to define the syntax and behavior of Imp
     _commands_ (or _statements_). *)
 
 (* ================================================================= *)
@@ -1273,8 +1306,11 @@ Proof. reflexivity. Qed.
 (** Informally, commands [c] are described by the following BNF
     grammar.
 
-     c := skip | x := a | c ; c | if b then c else c end
-         | while b do c end
+     c := skip
+        | x := a
+        | c ; c
+        | if b then c else c end
+        | while b do c end
 *)
 
 (** Here is the formal definition of the abstract syntax of
@@ -1299,14 +1335,16 @@ Notation "x := y"  :=
              y at level 85, no associativity) : com_scope.
 Notation "x ; y" :=
          (CSeq x y)
-           (in custom com at level 90, right associativity) : com_scope.
+           (in custom com at level 90,
+            right associativity) : com_scope.
 Notation "'if' x 'then' y 'else' z 'end'" :=
          (CIf x y z)
            (in custom com at level 89, x at level 99,
             y at level 99, z at level 99) : com_scope.
 Notation "'while' x 'do' y 'end'" :=
          (CWhile x y)
-            (in custom com at level 89, x at level 99, y at level 99) : com_scope.
+           (in custom com at level 89, x at level 99,
+            y at level 99) : com_scope.
 
 (** For example, here is the factorial function again, written as a
     formal Coq definition.  When this command terminates, the variable
@@ -1338,8 +1376,7 @@ Print fact_in_coq.
     - [Set Printing All] (undo with [Unset Printing All])
 
     These commands can also be used in the middle of a proof, to
-    elaborate the current goal and context.
- *)
+    elaborate the current goal and context. *)
 
 Unset Printing Notations.
 Print fact_in_coq.
@@ -1415,14 +1452,15 @@ Locate ";".
 Locate "while".
 (* ===>
     Notation
-      "'while' x 'do' y 'end'" := CWhile x y : com_scope (default interpretation)
-      "'_' '!->' v" := t_empty v (default interpretation)
+      "'while' x 'do' y 'end'" :=
+          CWhile x y : com_scope (default interpretation)
 *)
 
 (* ================================================================= *)
 (** ** More Examples *)
 
-(** Assignment: *)
+(* ----------------------------------------------------------------- *)
+(** *** Assignment: *)
 
 Definition plus2 : com :=
   <{ X := X + 2 }>.
@@ -1430,12 +1468,12 @@ Definition plus2 : com :=
 Definition XtimesYinZ : com :=
   <{ Z := X * Y }>.
 
+(* ----------------------------------------------------------------- *)
+(** *** Loops *)
+
 Definition subtract_slowly_body : com :=
   <{ Z := Z - 1 ;
      X := X - 1 }>.
-
-(* ----------------------------------------------------------------- *)
-(** *** Loops *)
 
 Definition subtract_slowly : com :=
   <{ while X <> 0 do
@@ -1465,8 +1503,8 @@ Definition loop : com :=
 (* ================================================================= *)
 (** ** Evaluation as a Function (Failed Attempt) *)
 
-(** Here's an attempt at defining an evaluation function for commands,
-    omitting the [while] case. *)
+(** Here's an attempt at defining an evaluation function for commands
+    (with a bogus [while] case). *)
 
 Fixpoint ceval_fun_no_while (st : state) (c : com) : state :=
   match c with
@@ -1616,7 +1654,7 @@ Inductive ceval : com -> state -> state -> Prop :=
   where "st =[ c ]=> st'" := (ceval c st st').
 
 (** The cost of defining evaluation as a relation instead of a
-    function is that we now need to construct _proofs_ that some
+    function is that we now need to construct a _proof_ that some
     program evaluates to some result state, rather than just letting
     Coq's computation mechanism do it for us. *)
 
@@ -1635,8 +1673,8 @@ Proof.
     apply E_Asgn. reflexivity.
   - (* if command *)
     apply E_IfFalse.
-    reflexivity.
-    apply E_Asgn. reflexivity.
+    + reflexivity.
+    + apply E_Asgn. reflexivity.
 Qed.
 
 (** **** Exercise: 2 stars, standard (ceval_example2) *)
@@ -1679,16 +1717,18 @@ Theorem pup_to_2_ceval :
   ]=> (X !-> 0 ; Y !-> 3 ; X !-> 1 ; Y !-> 2 ; Y !-> 0 ; X !-> 2).
 Proof.
   apply E_Seq with (Y !-> 0 ; X !-> 2).
-  apply E_Asgn. reflexivity.
-  apply E_WhileTrue with (X !-> 1 ; Y !-> 2 ; Y !-> 0 ; X !-> 2). reflexivity.
-  apply E_Seq with (Y !-> 2 ; Y !-> 0 ; X !-> 2).
-  apply E_Asgn. reflexivity.
-  apply E_Asgn. reflexivity.
-  apply E_WhileTrue with (X !-> 0 ; Y !-> 3 ; X !-> 1 ; Y !-> 2 ; Y !-> 0 ; X !-> 2). reflexivity.
-  apply E_Seq with (Y !-> 3 ; X !-> 1 ; Y !-> 2 ; Y !-> 0 ; X !-> 2).
-  apply E_Asgn. reflexivity.
-  apply E_Asgn. reflexivity.
-  apply E_WhileFalse. reflexivity.
+  - apply E_Asgn. reflexivity.
+  - apply E_WhileTrue with (X !-> 1 ; Y !-> 2 ; Y !-> 0 ; X !-> 2).
+    + reflexivity.
+    + apply E_Seq with (Y !-> 2 ; Y !-> 0 ; X !-> 2).
+      * apply E_Asgn. reflexivity.
+      * apply E_Asgn. reflexivity.
+    + apply E_WhileTrue with (X !-> 0 ; Y !-> 3 ; X !-> 1 ; Y !-> 2 ; Y !-> 0 ; X !-> 2).
+      * reflexivity.
+      * apply E_Seq with (Y !-> 3 ; X !-> 1 ; Y !-> 2 ; Y !-> 0 ; X !-> 2).
+        ** apply E_Asgn. reflexivity.
+        ** apply E_Asgn. reflexivity.
+      * apply E_WhileFalse. reflexivity.
 Qed.
 (** [] *)
 
@@ -1862,12 +1902,16 @@ Proof.
   - intros. exists st. constructor.
   - intros. exists (x !-> (aeval st a) ; st). constructor. reflexivity.
   - intros. inversion H as [| | c1' c2' H1 H2|]. subst. clear H.
-    assert (H: exists st1, st =[ c1 ]=> st1). apply IHc1. assumption. clear H1. destruct H as [st1 H1].
-    assert (H: exists st2, st1 =[ c2 ]=> st2). apply IHc2. assumption. clear H2. destruct H as [st2 H2].
+    assert (H: exists st1, st =[ c1 ]=> st1). { apply IHc1. assumption. }
+    clear H1. destruct H as [st1 H1].
+    assert (H: exists st2, st1 =[ c2 ]=> st2). { apply IHc2. assumption. }
+    clear H2. destruct H as [st2 H2].
     exists st2. apply E_Seq with (st':=st1); assumption.
   - intros. inversion H as [| | | b' c1' c2' H1 H2]. subst. clear H.
-    assert (H: exists st1, st =[ c1 ]=> st1). apply IHc1. assumption. clear H1. destruct H as [st1 H1].
-    assert (H: exists st2, st =[ c2 ]=> st2). apply IHc2. assumption. clear H2. destruct H as [st2 H2].
+    assert (H: exists st1, st =[ c1 ]=> st1). { apply IHc1. assumption. }
+    clear H1. destruct H as [st1 H1].
+    assert (H: exists st2, st =[ c2 ]=> st2). { apply IHc2. assumption. }
+    clear H2. destruct H as [st2 H2].
     destruct (beval st b) eqn:Hbeval.
     + exists st1. apply E_IfTrue; assumption.
     + exists st2. apply E_IfFalse; assumption.
@@ -2289,7 +2333,9 @@ Proof.
     subst.
   - rewrite contra in E'. discriminate.
   - exists st. assumption.
-  - apply IH. reflexivity. assumption.
+  - apply IH.
+    + reflexivity.
+    + assumption.
 Qed.
 (** [] *)
 
@@ -2309,13 +2355,27 @@ Proof.
     try (split; reflexivity);
     try (apply IHE1; assumption);
     try (rewrite H in H0; discriminate).
-  + destruct (IHE1 SContinue st'0). assumption. discriminate.
-  + destruct (IHE1_1 SBreak st2). assumption. discriminate.
-  + destruct (IHE1_1 SContinue st'0). assumption. subst. apply IHE1_2. assumption.
-  + split. apply IHE1 with SBreak. assumption. reflexivity.
-  + destruct (IHE1 SContinue st'0). assumption. discriminate.
-  + destruct (IHE1_1 SBreak st2). assumption. discriminate.
-  + destruct (IHE1_1 SContinue st'0). assumption. subst. apply IHE1_2. assumption.
+  + destruct (IHE1 SContinue st'0).
+    * assumption.
+    * discriminate.
+  + destruct (IHE1_1 SBreak st2).
+    * assumption.
+    * discriminate.
+  + destruct (IHE1_1 SContinue st'0).
+    * assumption.
+    * subst. apply IHE1_2. assumption.
+  + split.
+    * apply IHE1 with SBreak. assumption.
+    * reflexivity.
+  + destruct (IHE1 SContinue st'0).
+    * assumption.
+    * discriminate.
+  + destruct (IHE1_1 SBreak st2).
+    * assumption.
+    * discriminate.
+  + destruct (IHE1_1 SContinue st'0).
+    * assumption.
+    * subst. apply IHE1_2. assumption.
 Qed.
 
 (** [] *)
@@ -2431,15 +2491,29 @@ Proof.
     try (split; reflexivity);
     try (apply IHE1; assumption);
     try (rewrite H in H0; discriminate).
-  + destruct (IHE1 SContinue st'0). assumption. discriminate.
-  + destruct (IHE1_1 SBreak st2). assumption. discriminate.
-  + destruct (IHE1_1 SContinue st'0). assumption. subst. apply IHE1_2. assumption.
-  + split. apply IHE1 with SBreak. assumption. reflexivity.
-  + destruct (IHE1 SContinue st'0). assumption. discriminate.
-  + destruct (IHE1_1 SBreak st2). assumption. discriminate.
-  + destruct (IHE1_1 SContinue st'0). assumption. subst. apply IHE1_2. assumption.
+  + destruct (IHE1 SContinue st'0).
+    * assumption.
+    * discriminate.
+  + destruct (IHE1_1 SBreak st2).
+    * assumption.
+    * discriminate.
+  + destruct (IHE1_1 SContinue st'0).
+    * assumption.
+    * subst. apply IHE1_2. assumption.
+  + split.
+    * apply IHE1 with SBreak. assumption.
+    * reflexivity.
+  + destruct (IHE1 SContinue st'0).
+    * assumption.
+    * discriminate.
+  + destruct (IHE1_1 SBreak st2).
+    * assumption.
+    * discriminate.
+  + destruct (IHE1_1 SContinue st'0).
+    * assumption.
+    * subst. apply IHE1_2. assumption.
 Qed.
 
 End ForImp.
 
-(* 2022-08-08 17:13 *)
+(* 2025-01-13 16:00 *)
